fix one of the compat lemmas

rupicola/io/LogRelSourceTarget.CompatibilityLemmas.fst
@@ -1720,7 +1720,18 @@ let compat_oprod_pair #g
   end
 #pop-options
 
-#push-options "--z3rlimit 30 --split_queries always"
+let lem_fs_beh_return_inv (#t:qType) (val_:fs_val t) (h:history) (lt:local_trace h) (fs_r:fs_val t) :
+  Lemma (requires fs_beh (return val_) h lt fs_r)
+        (ensures lt == [] /\ fs_r == val_) =
+  theta_monad_morphism_ret val_;
+  assert (theta (io_return val_) == hist_return val_);
+  let p : hist_post h (get_Type t) = fun lt' r' -> lt' == [] /\ r' == val_ in
+  assert (hist_return val_ h p);
+  assert (theta (io_return val_) h p);
+  assert (thetaP (io_return val_) h lt fs_r);
+  assert (p lt fs_r)
+
+#push-options "--z3rlimit 100 --split_queries always"
 let helper_compat_oprod_string_eq_steps (h:history) (lt:local_trace h)
   (fs_e1':fs_prod qString) (fs_e2':fs_prod qString) (fs_r:fs_val qBool) (e1 e2:closed_exp) :
   Lemma
@@ -1740,7 +1751,6 @@ let helper_compat_oprod_string_eq_steps (h:history) (lt:local_trace h)
     returns exists e'. qBool ∈ (h++lt, fs_r, e') /\ e_beh (EStringEq e1 e2) e' h lt with _. begin
   lem_values_are_values qString (h++lt1) fs_v1 em1;
   lem_value_is_irred em1;
-  let EString s1 = em1 in
   // Decompose inner bind: fs_prod_bind fs_e2' (fun v2 -> return (fs_v1 = v2))
   let fs_k2 : fs_val qString -> fs_prod qBool = fun v2 -> return (fs_v1 = v2) in
   assert (fs_prod_bind #qString #qBool fs_e2' fs_k2 == io_bind fs_e2' fs_k2) by (norm [delta_only [`%fs_prod_bind]]; trefl ());
@@ -1748,13 +1758,8 @@ let helper_compat_oprod_string_eq_steps (h:history) (lt:local_trace h)
   eliminate exists (lt2a:local_trace (h++lt1)) (lt2b:local_trace ((h++lt1)++lt2a)) (fs_v2:fs_val qString).
     lt2 == (lt2a@lt2b) /\ fs_beh fs_e2' (h++lt1) lt2a fs_v2 /\ fs_beh (return (fs_v1 = fs_v2)) ((h++lt1)++lt2a) lt2b fs_r
     returns exists e'. qBool ∈ (h++lt, fs_r, e') /\ e_beh (EStringEq e1 e2) e' h lt with _. begin
-  let val_ : bool = (fs_v1 = fs_v2) in
-  theta_monad_morphism_ret val_;
-  let p : hist_post ((h++lt1)++lt2a) bool = fun lt' r' -> lt' == [] /\ r' == val_ in
-  assert (hist_return val_ ((h++lt1)++lt2a) p);
-  assert (theta (io_return val_) ((h++lt1)++lt2a) p);
-  assert (thetaP (io_return val_) ((h++lt1)++lt2a) lt2b fs_r);
-  assert (p lt2b fs_r);
+  let val_ = (fs_v1 = fs_v2) in
+  lem_fs_beh_return_inv #qBool val_ ((h++lt1)++lt2a) lt2b fs_r;
   assert (lt2b == []);
   assert (fs_r == val_);
   unit_l lt2a;
@@ -1765,18 +1770,26 @@ let helper_compat_oprod_string_eq_steps (h:history) (lt:local_trace h)
     returns exists e'. qBool ∈ (h++lt, fs_r, e') /\ e_beh (EStringEq e1 e2) e' h lt with _. begin
   lem_values_are_values qString ((h++lt1)++lt2a) fs_v2 em2;
   lem_value_is_irred em2;
-  let EString s2 = em2 in
   trans_history h lt1 lt2a;
   val_type_closed_under_history_extension qString (h++lt1) fs_v1 em1;
+  // em1 and em2 are string values
+  let EString s1 = em1 in
+  let EString s2 = em2 in
   let result = if s1 = s2 then ETrue else EFalse in
-  let _ : step (EStringEq (EString s1) (EString s2)) result (h++(lt1@lt2a)) None = StringEqReturn s1 s2 (h++(lt1@lt2a)) in
-  lem_step_implies_steps (EStringEq (EString s1) (EString s2)) result (h++(lt1@lt2a)) None;
+  let _ : step (EStringEq (EString s1) (EString s2)) result ((h++lt1)++lt2a) None = StringEqReturn s1 s2 ((h++lt1)++lt2a) in
+  lem_step_implies_steps (EStringEq (EString s1) (EString s2)) result ((h++lt1)++lt2a) None;
   lem_value_is_irred result;
-  // Construct: EStringEq e1 e2 -->* EStringEq (EString s1) (EString s2) --> result
+  // Pre-establish needed facts for the squash block
+  assert ((h++lt1)++lt2a == h++lt);
+  assert (steps (EStringEq (EString s1) (EString s2)) result (h++lt) []);
+  assert (indexed_irred em1 (h++lt1));
+  assert (indexed_irred em2 ((h++lt1)++lt2a));
+  // Construct: EStringEq e1 e2 -->* EStringEq em1 em2 --> result
   FStar.Squash.bind_squash #(steps e1 em1 h lt1) () (fun sts1 ->
   FStar.Squash.bind_squash #(steps e2 em2 (h++lt1) lt2a) () (fun sts2 ->
   construct_steps_estringeq e1 em1 e2 em2 h lt1 lt2a sts1 sts2;
-  lem_steps_transitive (EStringEq e1 e2) (EStringEq (EString s1) (EString s2)) result h (lt1@lt2a) []))
+  lem_steps_transitive (EStringEq e1 e2) (EStringEq (EString s1) (EString s2)) result h lt [];
+  unit_l lt))
   end
   end
   end
